Simplify things: use HeaderStateMap as a type for both input and output of the transformer.

CrSemantics.v
@@ -5,22 +5,28 @@ Import ListNotations.
 Require Import Strings.String.
 From MyProject Require Export CrIdentifiers.
 
+(* Code below is for efficient finite maps from the Rocq stdlib *)
+Require Import Coq.FSets.FMapAVL.
+Require Import Coq.Structures.OrderedTypeEx.
+Module StringMap := FMapAVL.Make(String_as_OT).
+Definition Dict := StringMap.t nat.
+
 
 (* Headers and states (or rather their valuations) are both represented
    as maps from names of headers and state variables to their values expressed as integers *)
-Definition HeaderMap := string -> nat.
-Definition StateMap := string -> nat.
+Definition HeaderMap := Dict.
+Definition StateMap := Dict.
 
 (* InputType is the input to the transformer, which is a pair of previous header and previous state *)
 (* OutputType is the output of the transformer, which is a pair of new header and new state *)
-Definition InputType := (HeaderMap * StateMap)%type.
-Definition OutputType := (HeaderMap * StateMap)%type.
-
+Definition HeaderStatePair := (HeaderMap * StateMap)%type.
+Example header_state_pair_example : HeaderStatePair :=
+  (StringMap.empty nat, StringMap.empty nat).
 (* TODO: fill out eval_transformer body at the end,
    right now, we are just specifying it as a function that
    goes from previous value of header+state
    to new value of header+state *)
-Parameter eval_transformer : Transformer -> InputType -> OutputType.
+Parameter eval_transformer : Transformer -> HeaderStatePair -> HeaderStatePair.
 
 (* A Transformer is a list of match-action rules,
    where each rule is either sequential or parallel,
@@ -29,16 +35,22 @@ Parameter eval_transformer : Transformer -> InputType -> OutputType.
 (* Function to evaluate a match-action rule,
    meaning header ops within an action are evaluated
    according to the type of the rule (sequential or parallel) *)
-Parameter eval_match_action_rule : MatchActionRule -> InputType -> OutputType.
+Parameter eval_match_action_rule : MatchActionRule -> HeaderStatePair -> HeaderStatePair.
 
 (* Function to evaluate a sequential match-action rule,
    meaning header ops within an action are evaluated sequentially *)
-Parameter eval_seq_rule : MatchActionRule -> InputType -> OutputType.
+Parameter eval_seq_rule : MatchActionRule -> HeaderStatePair -> HeaderStatePair.
 
 (* Function to evaluate a parallel match-action rule,
    meaning header ops within an action are evaluated in parallel *)
-Parameter eval_par_rule : MatchActionRule -> InputType -> OutputType.
+Parameter eval_par_rule : MatchActionRule -> HeaderStatePair -> HeaderStatePair.
 
 (* Function to evaluate a header operation,
    meaning we apply the operation to the header and state *)
-Parameter eval_hdr_op : HdrOp -> InputType -> OutputType.
+Definition eval_hdr_op (op : HdrOp) (input : HeaderStatePair) : HeaderStatePair :=
+    match op with
+    | StatefulOp f arg1 arg2 target => header_state_pair_example (* Placeholder for actual evaluation logic *)
+    | StatelessOp f arg1 arg2 target => header_state_pair_example (* Placeholder for actual evaluation logic *)
+    end.
+
+(*TODO: Maybe figure out a way to unify parsing and header manipulation into seq and par transformers respectively. *)
